Prove missing lemma from Examples

Kraken/Semantics.lean
@@ -655,34 +655,19 @@ def Directives.interp {α} [Undefined Bool α] [Throw α] [Labels]
 abbrev Program := List Directive
 abbrev Executable := Int64 × List (Directive × Nat) -- start and sizes
 
-class Layout where (start : Int64) (size : Nat → Nat)
+class Layout where
+  start : Int64
+  size : Nat → Nat
+
 def Layout.apply (l : Layout) (prog : Program) : Executable :=
   (l.start, prog.mapIdx (fun i d => (d, l.size i)))
+
 instance : CoeFun Layout (fun _ => Program → Executable) where coe := Layout.apply
 
--- TEMPORARY: delete when dropping support for Lean <= 4.28
--- (above which Init.Data.List.scan.Basic is supported).
--- This namespace permits use of Mathlib 4.27 which also implements its own
--- `scanl` which differs from the one here.
-namespace Kraken.Compat
-@[inline]
-private def scanAuxM {α β m} [Monad m] (f : β → α → m β) (init : β) (l : List α) : m (List β) :=
-  go l init []
-where
-  @[specialize] go : List α → β → List β → m (List β)
-    | [], last, acc => pure <| last :: acc
-    | x :: xs, last, acc => do go xs (← f last x) (last :: acc)
-@[inline]
-def scanlM {α β m} [Monad m] (f : β → α → m β) (init : β) (l : List α) : m (List β) :=
-  List.reverse <$> scanAuxM f init l
-@[inline]
-def scanl {α β} (f : β → α → β) (init : β) (as : List α) : List β :=
-  Id.run <| Kraken.Compat.scanlM (pure <| f · ·) init as
-end Kraken.Compat
-
 def Executable.withAddresses (e : Executable)  : List (Int64 × Directive × Nat) :=
-  (Kraken.Compat.scanl (fun (p, _, _) (d, z) => (p+.ofNat z, d, z)) (e.1, .byteArray (.mk #[]), 0) e.2)
+  (List.scanl (fun (p, _, _) (d, z) => (p+.ofNat z, d, z)) (e.1, .byteArray (.mk #[]), 0) e.2)
 
+@[reducible]
 def Executable.labels (e : Executable) : Labels :=
   { label l := (e.withAddresses.findSome?
       (fun (p, d, _) => if d = .label l then .some p else .none)).getD (-1) }
